pancake/semantics/crepSemScript.sml
@@ -248,9 +248,8 @@ Definition evaluate_def:
             (case call_FFI s.ffi (explode ffi_index) bytes bytes2 of
               | FFI_final outcome => (SOME (FinalFFI outcome),s)
               | FFI_return new_ffi new_bytes =>
-                (case write_bytearray w4 new_bytes s.memory s.memaddrs s.be of
-                  | SOME m => (NONE, s with <| memory := m;ffi := new_ffi |>)
-                  | NONE => (SOME Error,s)))
+                let nmem = write_bytearray w4 new_bytes s.memory s.memaddrs s.be in
+                  (NONE, s with <| memory := nmem; ffi := new_ffi |>))
          | _ => (SOME Error,s))
        | res => (SOME Error,s))
 Termination
